Several syntax beautifications

CFGraph/HOLCFAbsCF.thy
@@ -6,25 +6,21 @@ default_sort type
 
 consts abs :: "'a \<Rightarrow> 'b" ("|_|")
 
-setup {*
-  Adhoc_Overloading.add_overloaded @{const_name abs}
-*}
+setup {* Adhoc_Overloading.add_overloaded @{const_name abs} *}
 
 class contour = discrete_cpo +
-  fixes nb :: "'a \<Rightarrow> label \<Rightarrow> 'a"
-    and initial_contour :: 'a
-    and abs_cnt :: "HOLCFExCF.contour \<Rightarrow> 'a"
-  assumes abs_cnt_nb: "abs_cnt b \<sqsubseteq> b_a \<Longrightarrow> abs_cnt (HOLCFExCF.nb b lab) \<sqsubseteq> nb b_a lab"
-     and abs_cnt_initial[simp]: "abs_cnt(\<binit>) = initial_contour"
+  fixes nb_a :: "'a \<Rightarrow> label \<Rightarrow> 'a" ("\<anb>")
+    and a_initial_contour :: 'a ("\<abinit>")
+    and abs_cnt :: "contour \<Rightarrow> 'a"
+  assumes abs_cnt_nb: "abs_cnt b \<sqsubseteq> b_a \<Longrightarrow> abs_cnt (nb b lab) \<sqsubseteq> \<anb> b_a lab"
+     and abs_cnt_initial[simp]: "abs_cnt(\<binit>) = \<abinit>"
 
-setup {*
-  Adhoc_Overloading.add_variant @{const_name abs} @{const_name abs_cnt}
-*}
+setup {* Adhoc_Overloading.add_variant @{const_name abs} @{const_name abs_cnt} *}
 
 instantiation unit :: contour
 begin
-definition "nb _ _ = ()"
-definition "initial_contour = ()"
+definition "\<anb> _ _ = ()"
+definition "\<abinit> = ()"
 definition "abs_cnt _ = ()"
 instance by default auto
 end
@@ -57,9 +53,7 @@ text {* Abstraction functions *}
 definition abs_benv :: "HOLCFExCF.benv \<Rightarrow> 'c::contour benv"
   where "abs_benv \<beta> = Option.map abs_cnt \<circ> \<beta>"
 
-setup {*
-  Adhoc_Overloading.add_variant @{const_name abs} @{const_name abs_benv}
-*}
+setup {* Adhoc_Overloading.add_variant @{const_name abs} @{const_name abs_benv} *}
 
 lemma abs_benv_empty[simp]: "|empty| = empty"
 unfolding abs_benv_def by simp
@@ -70,9 +64,7 @@ lemma abs_benv_upd[simp]: "|\<beta>(c\<mapsto>b)| = |\<beta>| (c \<mapsto> |b| )
 primrec abs_closure :: "HOLCFExCF.closure \<Rightarrow> 'c::contour closure"
   where "abs_closure (l,\<beta>) = (l,|\<beta>| )"
 
-setup {*
-  Adhoc_Overloading.add_variant @{const_name abs} @{const_name abs_closure}
-*}
+setup {* Adhoc_Overloading.add_variant @{const_name abs} @{const_name abs_closure} *}
 
 primrec abs_d :: "HOLCFExCF.d \<Rightarrow> 'c::contour d"
   where "abs_d (DI i) = {}"
@@ -80,9 +72,7 @@ primrec abs_d :: "HOLCFExCF.d \<Rightarrow> 'c::contour d"
       | "abs_d (DC cl) = {PC |cl|}"
       | "abs_d (HOLCFExCF.Stop) = {Stop}"
 
-setup {*
-  Adhoc_Overloading.add_variant @{const_name abs} @{const_name abs_d}
-*}
+setup {* Adhoc_Overloading.add_variant @{const_name abs} @{const_name abs_d} *}
 
 lemma contents_is_Proc:
   assumes "isProc cnt"
@@ -92,18 +82,16 @@ using assms by (cases cnt)auto
 definition abs_venv :: "HOLCFExCF.venv \<Rightarrow> 'c::contour venv"
   where "abs_venv ve = (\<lambda>(v,b_a). \<Union>{(case ve (v,b) of Some d \<Rightarrow> |d| | None \<Rightarrow> {}) | b. |b| = b_a })"
 
-setup {*
-  Adhoc_Overloading.add_variant @{const_name abs} @{const_name abs_venv}
-*}
+setup {* Adhoc_Overloading.add_variant @{const_name abs} @{const_name abs_venv} *}
 
-fun evalV :: "val \<Rightarrow> 'c benv \<Rightarrow> 'c venv \<Rightarrow> 'c d"
-  where "evalV (C _ i) \<beta> ve = {}"
-  |     "evalV (P prim) \<beta> ve = {PP prim}"
-  |     "evalV (R _ var) \<beta> ve =
+fun evalV_a :: "val \<Rightarrow> 'c benv \<Rightarrow> 'c venv \<Rightarrow> 'c d" ("\<aA>")
+  where "\<aA> (C _ i) \<beta> ve = {}"
+  |     "\<aA> (P prim) \<beta> ve = {PP prim}"
+  |     "\<aA> (R _ var) \<beta> ve =
            (case \<beta> (binder var) of
               Some l \<Rightarrow> ve (var,l)
             | None \<Rightarrow> {})"
-  |     "evalV (L lam) \<beta> ve = {PC (lam, \<beta>)}"
+  |     "\<aA> (L lam) \<beta> ve = {PC (lam, \<beta>)}"
 
 types 'c ccache = "((label \<times> 'c benv) \<times> 'c proc) set"
       'c ans = "'c ccache"
@@ -113,9 +101,7 @@ definition abs_ccache :: "HOLCFExCF.ccache \<Rightarrow> 'c::contour ccache"
 (* equivalent, but I already have cont2cont for UNION
   where "abs_ccache cc = { ((c,abs_benv \<beta>),p) | c \<beta> p d . ((c,\<beta>),d) \<in> cc \<and> p \<in> abs_d d}" *)
 
-setup {*
-  Adhoc_Overloading.add_variant @{const_name abs} @{const_name abs_ccache}
-*}
+setup {* Adhoc_Overloading.add_variant @{const_name abs} @{const_name abs_ccache} *}
 
 types 'c fstate = "('c proc \<times> 'c d list \<times> 'c venv \<times> 'c)"
       'c cstate = "(call \<times> 'c benv \<times> 'c venv \<times> 'c)"
@@ -123,16 +109,12 @@ types 'c fstate = "('c proc \<times> 'c d list \<times> 'c venv \<times> 'c)"
 fun abs_fstate :: "HOLCFExCF.fstate \<Rightarrow> 'c::contour fstate"
   where "abs_fstate (d,ds,ve,b) = (contents |d|, map abs_d ds, |ve|, |b| )"
 
-setup {*
-  Adhoc_Overloading.add_variant @{const_name abs} @{const_name abs_fstate}
-*}
+setup {* Adhoc_Overloading.add_variant @{const_name abs} @{const_name abs_fstate} *}
 
 fun abs_cstate :: "HOLCFExCF.cstate \<Rightarrow> 'c::contour cstate"
   where "abs_cstate (c,\<beta>,ve,b) = (c, |\<beta>|, |ve|, |b| )"
 
-setup {*
-  Adhoc_Overloading.add_variant @{const_name abs} @{const_name abs_cstate}
-*}
+setup {* Adhoc_Overloading.add_variant @{const_name abs} @{const_name abs_cstate} *}
 
 lemma cont2cont_lambda_case [simp, cont2cont]:
   assumes "\<And>a b c. cont (\<lambda>x. f x a b c)"
@@ -162,37 +144,37 @@ lemma cont2cont_prim_case [simp, cont2cont]:
 using assms
 by (cases p) auto
 
-lemma abs_venv_empty[simp]: "|empty| = smap_empty"
+lemma abs_venv_empty[simp]: "|empty| = {}."
   apply (rule ext) by (auto simp add: abs_venv_def smap_empty_def)
 
-lemma abs_venv_union: "\<And> ve1 ve2. |ve1 ++ ve2| \<sqsubseteq> smap_union |ve1| |ve2|"
+lemma abs_venv_union: "\<And> ve1 ve2. |ve1 ++ ve2| \<sqsubseteq> |ve1| \<union>. |ve2|"
   by (subst below_fun_def, auto simp add: sqsubset_is_subset abs_venv_def smap_union_def, split option.split_asm, auto)
 
-lemma abs_venv_map_of_rev: "|map_of (rev l)| \<sqsubseteq> smap_Union (map (\<lambda>(v,k). |[v \<mapsto> k]| ) l)"
+lemma abs_venv_map_of_rev: "|map_of (rev l)| \<sqsubseteq> \<Union>. (map (\<lambda>(v,k). |[v \<mapsto> k]| ) l)"
 proof (induct l)
   case Nil show ?case unfolding abs_venv_def by (subst below_fun_def, auto simp: sqsubset_is_subset) next
   case (Cons a l)
     obtain v k where "a=(v,k)" by (rule prod.exhaust)
-    hence "|map_of (rev (a#l))| \<sqsubseteq> (smap_union |[v \<mapsto> k]| |map_of (rev l)| :: 'a venv)"
+    hence "|map_of (rev (a#l))| \<sqsubseteq> |[v \<mapsto> k]| \<union>. |map_of (rev l)| :: 'a venv"
       by (auto intro: abs_venv_union)
     also
-    have "\<dots> \<sqsubseteq> smap_union | [v \<mapsto> k] | (smap_Union (map (\<lambda>(v,k). |[v  \<mapsto> k]| ) l))"
+    have "\<dots> \<sqsubseteq> |[v \<mapsto> k]| \<union>. (\<Union>. (map (\<lambda>(v,k). |[v  \<mapsto> k]| ) l))"
       by (rule smap_union_mono[OF below_refl Cons])
     also
-    have "\<dots> = smap_Union ( |[v \<mapsto> k]| # map (\<lambda>(v,k). |[v \<mapsto> k]| ) l)"
+    have "\<dots> = \<Union>. ( |[v \<mapsto> k]| # map (\<lambda>(v,k). |[v \<mapsto> k]| ) l)"
       by (rule smap_Union_union)
     also
-    have "\<dots> = smap_Union (map (\<lambda>(v,k). |[v \<mapsto> k]| ) (a#l))"
+    have "\<dots> = \<Union>. (map (\<lambda>(v,k). |[v \<mapsto> k]| ) (a#l))"
       using `a = (v,k)`
       by auto 
     finally
     show ?case .
 qed
 
-lemma abs_venv_map_of: "|map_of l| \<sqsubseteq> smap_Union (map (\<lambda>(v,k). |[v \<mapsto> k]| ) l)"
+lemma abs_venv_map_of: "|map_of l| \<sqsubseteq> \<Union>. (map (\<lambda>(v,k). |[v \<mapsto> k]| ) l)"
   using abs_venv_map_of_rev[of "rev l"] by simp
 
-lemma abs_venv_singleton: "|[(v,b) \<mapsto> d]| = smap_singleton (v,|b| ) |d|"
+lemma abs_venv_singleton: "|[(v,b) \<mapsto> d]| = {(v,|b| ) := |d|}."
   by (rule ext, auto simp add:abs_venv_def smap_singleton_def smap_empty_def)
 
 lemma abs_ccache_union: "|c1 \<union> c2| \<sqsubseteq> |c1| \<union> |c2|"
@@ -205,7 +187,7 @@ lemma abs_cache_singleton [simp]: "|{((c,\<beta>),d)}| = {((c, |\<beta>| ), p) |
 
 lemma abs_d_evalV:
   assumes "|ve::HOLCFExCF.venv| \<sqsubseteq> ve_a"
-  shows "|HOLCFExCF.evalV f \<beta> ve| \<subseteq> HOLCFAbsCF.evalV f |\<beta>| ve_a"
+  shows "|\<A> f \<beta> ve| \<subseteq> \<aA> f |\<beta>| ve_a"
 proof(cases f)
 case (R _ v)
   from assms have assm': "\<And>v b. option_case {} abs_d (ve (v,b))  \<subseteq> ve_a (v,|b| )"
@@ -221,51 +203,51 @@ qed auto
 
 lemma lemma7:
   assumes "|ve::HOLCFExCF.venv| \<sqsubseteq> ve_a"
-  shows "|HOLCFExCF.evalV a \<beta> ve| \<sqsubseteq> evalV a |\<beta>| ve_a"
+  shows "|\<A> a \<beta> ve| \<sqsubseteq> \<aA> a |\<beta>| ve_a"
 using assms
  by (subst sqsubset_is_subset, rule abs_d_evalV)
 
-fixrec   evalF :: "'c::contour fstate discr \<rightarrow> 'c ans"
-     and evalC :: "'c::contour cstate discr \<rightarrow> 'c ans"
-  where "evalF\<cdot>fstate = (case undiscr fstate of
+fixrec   evalF :: "'c::contour fstate discr \<rightarrow> 'c ans" ("\<aF>")
+     and evalC :: "'c::contour cstate discr \<rightarrow> 'c ans" ("\<aC>")
+  where "\<aF>\<cdot>fstate = (case undiscr fstate of
              (PC (Lambda lab vs c, \<beta>), as, ve, b) \<Rightarrow>
                (if length vs = length as
                 then let \<beta>' = \<beta> (lab \<mapsto> b);
-                         ve' = smap_union ve (smap_Union (map (\<lambda>(v,a). smap_singleton (v,b) a) (zip vs as)))
-                     in evalC\<cdot>(Discr (c,\<beta>',ve',b))
+                         ve' = ve \<union>. (\<Union>. (map (\<lambda>(v,a). {(v,b) := a}.) (zip vs as)))
+                     in \<aC>\<cdot>(Discr (c,\<beta>',ve',b))
                 else \<bottom>)
             | (PP (Plus c),[_,_,cnts],ve,b) \<Rightarrow>
-                     let b' = nb b c;
+                     let b' = \<anb> b c;
                          \<beta>  = [c \<mapsto> b]
-                     in (\<Union>cnt\<in>cnts. evalF\<cdot>(Discr (cnt,[{}],ve,b')))
+                     in (\<Union>cnt\<in>cnts. \<aF>\<cdot>(Discr (cnt,[{}],ve,b')))
                         \<union>
                         {((c, \<beta>), cont) | cont . cont \<in> cnts}
             | (PP (prim.If ct cf),[_, cntts, cntfs],ve,b) \<Rightarrow>
-                  ((   let b' = nb b ct;
+                  ((   let b' = \<anb> b ct;
                             \<beta> = [ct \<mapsto> b]
-                        in (\<Union>cnt\<in>cntts . evalF\<cdot>(Discr (cnt,[],ve,b')))
+                        in (\<Union>cnt\<in>cntts . \<aF>\<cdot>(Discr (cnt,[],ve,b')))
                            \<union>{((ct, \<beta>), cnt) | cnt . cnt \<in> cntts}
                    )\<union>(
-                       let b' = nb b cf;
+                       let b' = \<anb> b cf;
                             \<beta> = [cf \<mapsto> b]
-                        in (\<Union>cnt\<in>cntfs . evalF\<cdot>(Discr (cnt,[],ve,b')))
+                        in (\<Union>cnt\<in>cntfs . \<aF>\<cdot>(Discr (cnt,[],ve,b')))
                            \<union>{((cf, \<beta>), cnt) | cnt . cnt \<in> cntfs}
                    ))
             | (Stop,[_],_,_) \<Rightarrow> {}
             | _ \<Rightarrow> \<bottom>
         )"
-      | "evalC\<cdot>cstate = (case undiscr cstate of
+      | "\<aC>\<cdot>cstate = (case undiscr cstate of
              (App lab f vs,\<beta>,ve,b) \<Rightarrow>
-                 let fs = evalV f \<beta> ve;
-                     as = map (\<lambda>v. evalV v \<beta> ve) vs;
-                     b' = nb b lab
-                  in (\<Union>f' \<in> fs. evalF\<cdot>(Discr (f',as,ve,b')))
+                 let fs = \<aA> f \<beta> ve;
+                     as = map (\<lambda>v. \<aA> v \<beta> ve) vs;
+                     b' = \<anb> b lab
+                  in (\<Union>f' \<in> fs. \<aF>\<cdot>(Discr (f',as,ve,b')))
                      \<union>{((lab, \<beta>),f') | f' . f'\<in> fs}
             | (Let lab ls c',\<beta>,ve,b) \<Rightarrow>
-                 let b' = nb b lab;
+                 let b' = \<anb> b lab;
                      \<beta>' = \<beta> (lab \<mapsto> b');
-                     ve' = smap_union ve (smap_Union (map (\<lambda>(v,l). smap_singleton (v,b') (evalV (L l) \<beta>' ve)) ls))
-                 in evalC\<cdot>(Discr (c',\<beta>',ve',b'))
+                     ve' = ve \<union>. (\<Union>. (map (\<lambda>(v,l). {(v,b') := (\<aA> (L l) \<beta>' ve)}.) ls))
+                 in \<aC>\<cdot>(Discr (c',\<beta>',ve',b'))
         )"
 
 print_theorems
@@ -289,8 +271,8 @@ using assms
 by (rule cont2cont)(rule cont_const)
 
 lemma lemma89:
- shows "|fstate| \<sqsubseteq> (fstate_a::'c::contour fstate) \<Longrightarrow> |HOLCFExCF.evalF\<cdot>(Discr fstate)| \<sqsubseteq> evalF\<cdot>(Discr fstate_a)"
-   and "|cstate| \<sqsubseteq> (cstate_a::'c::contour cstate) \<Longrightarrow> |HOLCFExCF.evalC\<cdot>(Discr cstate)| \<sqsubseteq> evalC\<cdot>(Discr cstate_a)" 
+ shows "|fstate| \<sqsubseteq> (fstate_a::'c::contour fstate) \<Longrightarrow> |\<F>\<cdot>(Discr fstate)| \<sqsubseteq> \<aF>\<cdot>(Discr fstate_a)"
+   and "|cstate| \<sqsubseteq> (cstate_a::'c::contour cstate) \<Longrightarrow> |\<C>\<cdot>(Discr cstate)| \<sqsubseteq> \<aC>\<cdot>(Discr cstate_a)"
 proof(induct arbitrary: fstate fstate_a cstate cstate_a rule: HOLCFExCF.evalF_evalC_induct)
 print_cases
 case Admissibility show ?case
@@ -328,36 +310,36 @@ case (Next evalF evalC) {
   moreover
 
   { have "|ve(map (\<lambda>v. (v, b)) vs [\<mapsto>] ds)|
-          \<sqsubseteq> smap_union |ve| |map_of (rev (zip (map (\<lambda>v. (v, b)) vs) ds))|"
+          \<sqsubseteq> |ve| \<union>. |map_of (rev (zip (map (\<lambda>v. (v, b)) vs) ds))|"
       unfolding map_upds_def by (intro abs_venv_union)
     also
-    have "\<dots> \<sqsubseteq> smap_union ve_a (smap_Union (map (\<lambda>(v,k). |[v \<mapsto> k]| ) (zip (map (\<lambda>v. (v, b)) vs) ds)))"
+    have "\<dots> \<sqsubseteq> ve_a  \<union>. (\<Union>. (map (\<lambda>(v,k). |[v \<mapsto> k]| ) (zip (map (\<lambda>v. (v, b)) vs) ds)))"
       by (rule smap_union_mono[OF abs_ve abs_venv_map_of_rev])
     also
-    have "\<dots> = smap_union ve_a (smap_Union (map (\<lambda>(v,y). |[(v,b) \<mapsto> y]| ) (zip vs ds)))"
+    have "\<dots> = ve_a \<union>. (\<Union>. (map (\<lambda>(v,y). |[(v,b) \<mapsto> y]| ) (zip vs ds)))"
       by (auto simp add: zip_map1 o_def split_def)
     also
-    have "\<dots> \<sqsubseteq> smap_union ve_a (smap_Union (map (\<lambda>(v,y). smap_singleton (v, b_a) y) (zip vs ds_a)))"
+    have "\<dots> \<sqsubseteq> ve_a \<union>. (\<Union>. (map (\<lambda>(v,y). {(v,b_a) := y}.) (zip vs ds_a)))"
     proof-
       from abs_b abs_ds
       have"list_all2 op \<sqsubseteq> (map (\<lambda>(v, y). |[(v, b) \<mapsto> y]| ) (zip vs ds))
-                          (map (\<lambda>(v, y). smap_singleton (v, b_a) y) (zip vs ds_a))"
+                          (map (\<lambda>(v, y). {(v,b_a) := y}.) (zip vs ds_a))"
       by (auto simp add: abs_venv_singleton below_list_def list_all2_conv_all_nth intro:smap_singleton_mono list_all2I)
       thus ?thesis
         by(rule smap_union_mono[OF below_refl smap_Union_mono])
     qed
     finally
     have "|ve(map (\<lambda>v. (v, b)) vs [\<mapsto>] ds)|
-          \<sqsubseteq> smap_union ve_a (smap_Union (map (\<lambda>(v,y). smap_singleton (v, b_a) y) (zip vs ds_a)))".
+          \<sqsubseteq> ve_a \<union>. (\<Union>. (map (\<lambda>(v,y). {(v, b_a) := y}.) (zip vs ds_a)))".
   }
   ultimately
   have prem: "|(c, \<beta>(lab \<mapsto> b), ve(map (\<lambda>v. (v, b)) vs [\<mapsto>] ds), b)|
-        \<sqsubseteq> (c,  |\<beta>|(lab \<mapsto> b_a), smap_union ve_a (smap_Union(map (\<lambda>(v, y). smap_singleton (v, b_a) y) (zip vs ds_a))), b_a)"
+        \<sqsubseteq> (c,  |\<beta>|(lab \<mapsto> b_a), ve_a \<union>. (\<Union>.(map (\<lambda>(v, y). {(v, b_a) := y}.) (zip vs ds_a))), b_a)"
     using abs_b
     by(auto simp only:Pair_below_iff abs_cstate.simps)
 
   show "|evalC\<cdot>(Discr (c, \<beta>(lab \<mapsto> b), ve(map (\<lambda>v. (v, b)) vs [\<mapsto>] ds), b))|
-        \<sqsubseteq> HOLCFAbsCF.evalF\<cdot>(Discr (PC (Lambda lab vs c, |\<beta>| ), ds_a, ve_a, b_a))"
+        \<sqsubseteq> \<aF>\<cdot>(Discr (PC (Lambda lab vs c, |\<beta>| ), ds_a, ve_a, b_a))"
   using Next.hyps(2)[OF prem] ds_a_length
   by (subst HOLCFAbsCF.evalF.simps, simp del:HOLCFAbsCF.evalF.simps HOLCFAbsCF.evalC.simps)
 
@@ -373,34 +355,34 @@ case (Next evalF evalC) {
     using abs_cnt and abs_b
     by (auto simp add:sqsubset_is_subset)
 
-  have prem: "|(cnt, [DI (a1 + a2)], ve, HOLCFExCF.nb b lab)| \<sqsubseteq>
-              (contents |cnt|, [{}], ve_a, contour_class.nb b_a lab)"
+  have prem: "|(cnt, [DI (a1 + a2)], ve, nb b lab)| \<sqsubseteq>
+              (contents |cnt|, [{}], ve_a, \<anb> b_a lab)"
     using abs_ve and abs_cnt_nb[OF abs_b]
     by (simp)
-  have "|(evalF\<cdot>(Discr (cnt, [DI (a1 + a2)], ve, HOLCFExCF.nb b lab)))|
-       \<sqsubseteq> HOLCFAbsCF.evalF\<cdot>(Discr (contents |cnt|, [{}], ve_a, contour_class.nb b_a lab))"
+  have "|(evalF\<cdot>(Discr (cnt, [DI (a1 + a2)], ve, nb b lab)))|
+       \<sqsubseteq> \<aF>\<cdot>(Discr (contents |cnt|, [{}], ve_a, \<anb> b_a lab))"
     by (rule Next.hyps(1)[OF prem])
-  also have "\<dots> \<sqsubseteq> (\<Union>cnt\<in>cnt_a. HOLCFAbsCF.evalF\<cdot>(Discr (cnt, [{}], ve_a, contour_class.nb b_a lab)))"
+  also have "\<dots> \<sqsubseteq> (\<Union>cnt\<in>cnt_a. \<aF>\<cdot>(Discr (cnt, [{}], ve_a, \<anb> b_a lab)))"
     using abs_cnt
     by (auto intro: contents_is_Proc[OF `isProc cnt`] simp del: evalF.simps simp add:sqsubset_is_subset)
   finally
-  have old_elems: "|(evalF\<cdot>(Discr (cnt, [DI (a1 + a2)], ve, HOLCFExCF.nb b lab)))|
-       \<sqsubseteq> (\<Union>cnt\<in>cnt_a. HOLCFAbsCF.evalF\<cdot>(Discr (cnt, [{}], ve_a, contour_class.nb b_a lab)))".
+  have old_elems: "|(evalF\<cdot>(Discr (cnt, [DI (a1 + a2)], ve, nb b lab)))|
+       \<sqsubseteq> (\<Union>cnt\<in>cnt_a. \<aF>\<cdot>(Discr (cnt, [{}], ve_a, \<anb> b_a lab)))".
    
-  have "|((evalF\<cdot>(Discr (cnt, [DI (a1 + a2)], ve, HOLCFExCF.nb b lab)))
+  have "|((evalF\<cdot>(Discr (cnt, [DI (a1 + a2)], ve, nb b lab)))
           \<union> {((lab, [lab \<mapsto> b]), cnt)})|
-        \<sqsubseteq> |(evalF\<cdot>(Discr (cnt, [DI (a1 + a2)], ve, HOLCFExCF.nb b lab)))|
+        \<sqsubseteq> |(evalF\<cdot>(Discr (cnt, [DI (a1 + a2)], ve, nb b lab)))|
           \<union> |{((lab, [lab \<mapsto> b]), cnt)}|"
     by (rule abs_ccache_union)
   also
   have "\<dots> \<sqsubseteq>
-        (\<Union>cnt\<in>cnt_a. HOLCFAbsCF.evalF\<cdot>(Discr (cnt, [{}], ve_a, contour_class.nb b_a lab)))
+        (\<Union>cnt\<in>cnt_a. \<aF>\<cdot>(Discr (cnt, [{}], ve_a, \<anb> b_a lab)))
         \<union> {((lab, [lab \<mapsto> b_a]), cont) |cont. cont \<in> cnt_a}"
     by (rule Un_mono_sq[OF old_elems new_elem])
   finally
   show "|insert ((lab, [lab \<mapsto> b]), cnt)
-                (evalF\<cdot>(Discr (cnt, [DI (a1 + a2)], ve, HOLCFExCF.nb b lab)))|
-        \<sqsubseteq> HOLCFAbsCF.evalF\<cdot>(Discr (PP (prim.Plus lab), ds_a, ve_a, b_a))"
+                (evalF\<cdot>(Discr (cnt, [DI (a1 + a2)], ve, nb b lab)))|
+        \<sqsubseteq> \<aF>\<cdot>(Discr (PP (prim.Plus lab), ds_a, ve_a, b_a))"
     using ds_a by (subst HOLCFAbsCF.evalF.simps)(auto simp del:HOLCFAbsCF.evalF.simps)
   next
 
@@ -419,43 +401,43 @@ case (Next evalF evalC) {
   have new_elem: "|{((?c, [?c \<mapsto> b]), ?cnt)}| \<sqsubseteq> {((?c, [?c \<mapsto> b_a]), cont) |cont. cont \<in> ?cnt_a}"
     using abs_cntt and abs_cntf and abs_b by (auto simp add:sqsubset_is_subset)
 
-  have prem: "|(?cnt, [], ve, HOLCFExCF.nb b ?c)| \<sqsubseteq>
-              (contents |?cnt|, [], ve_a, contour_class.nb b_a ?c)"
+  have prem: "|(?cnt, [], ve, nb b ?c)| \<sqsubseteq>
+              (contents |?cnt|, [], ve_a, \<anb> b_a ?c)"
     using abs_ve and abs_cnt_nb[OF abs_b]
     by (simp)
-  have "|evalF\<cdot>(Discr (?cnt, [], ve, HOLCFExCF.nb b ?c))|
-       \<sqsubseteq> HOLCFAbsCF.evalF\<cdot>(Discr (contents |?cnt|, [], ve_a, contour_class.nb b_a ?c))"
+  have "|evalF\<cdot>(Discr (?cnt, [], ve, nb b ?c))|
+       \<sqsubseteq> \<aF>\<cdot>(Discr (contents |?cnt|, [], ve_a, \<anb> b_a ?c))"
     by (rule Next.hyps(1)[OF prem])
-  also have "\<dots> \<sqsubseteq> (\<Union>cnt\<in>?cnt_a. HOLCFAbsCF.evalF\<cdot>(Discr (cnt, [], ve_a, contour_class.nb b_a ?c)))"
+  also have "\<dots> \<sqsubseteq> (\<Union>cnt\<in>?cnt_a. \<aF>\<cdot>(Discr (cnt, [], ve_a, \<anb> b_a ?c)))"
     using abs_cntt and abs_cntf
     by (auto intro: contents_is_Proc[OF `isProc ?cnt`] simp del: evalF.simps simp add:sqsubset_is_subset)
 
   finally
-  have old_elems: "|evalF\<cdot>(Discr (?cnt, [], ve, HOLCFExCF.nb b ?c))|
-       \<sqsubseteq> (\<Union>cnt\<in>?cnt_a. HOLCFAbsCF.evalF\<cdot>(Discr (cnt, [], ve_a, contour_class.nb b_a ?c)))".
+  have old_elems: "|evalF\<cdot>(Discr (?cnt, [], ve, nb b ?c))|
+       \<sqsubseteq> (\<Union>cnt\<in>?cnt_a. \<aF>\<cdot>(Discr (cnt, [], ve_a, \<anb> b_a ?c)))".
 
-  have "|evalF\<cdot>(Discr (?cnt, [], ve, HOLCFExCF.nb b ?c))
+  have "|evalF\<cdot>(Discr (?cnt, [], ve, nb b ?c))
           \<union> {((?c, [?c \<mapsto> b]), ?cnt)}|
-        \<sqsubseteq> |evalF\<cdot>(Discr (?cnt, [], ve, HOLCFExCF.nb b ?c))|
+        \<sqsubseteq> |evalF\<cdot>(Discr (?cnt, [], ve, nb b ?c))|
           \<union> |{((?c, [?c \<mapsto> b]), ?cnt)}|"
     by (rule abs_ccache_union)
   also
   have "\<dots> \<sqsubseteq>
-        (\<Union>cnt\<in>?cnt_a. HOLCFAbsCF.evalF\<cdot>(Discr (cnt, [], ve_a, contour_class.nb b_a ?c)))
+        (\<Union>cnt\<in>?cnt_a. \<aF>\<cdot>(Discr (cnt, [], ve_a, \<anb> b_a ?c)))
         \<union> {((?c, [?c \<mapsto> b_a]), cont) |cont. cont \<in> ?cnt_a}"
     by (rule Un_mono_sq[OF old_elems new_elem])
   also
   have "\<dots> \<sqsubseteq> 
-        ((\<Union>cnt\<in>cntt_a. HOLCFAbsCF.evalF\<cdot>(Discr (cnt, [], ve_a, contour_class.nb b_a ct)))
+        ((\<Union>cnt\<in>cntt_a. \<aF>\<cdot>(Discr (cnt, [], ve_a, \<anb> b_a ct)))
           \<union> {((ct, [ct \<mapsto> b_a]), cont) |cont. cont \<in> cntt_a})
-      \<union> ((\<Union>cnt\<in>cntf_a. HOLCFAbsCF.evalF\<cdot>(Discr (cnt, [], ve_a, contour_class.nb b_a cf)))
+      \<union> ((\<Union>cnt\<in>cntf_a. \<aF>\<cdot>(Discr (cnt, [], ve_a, \<anb> b_a cf)))
           \<union> {((cf, [cf \<mapsto> b_a]), cont) |cont. cont \<in> cntf_a})"
     by (rule subst[OF sqsubset_is_subset[THEN sym],of "\<lambda>x. x",OF Un_upper1]
        |rule subst[OF sqsubset_is_subset[THEN sym],of "\<lambda>x. x",OF Un_upper2])
   finally
   show "|insert ((?c, [?c \<mapsto> b]), ?cnt)
-                (evalF\<cdot>(Discr (?cnt, [], ve, HOLCFExCF.nb b ?c)))| \<sqsubseteq>
-          HOLCFAbsCF.evalF\<cdot>(Discr (PP (prim.If ct cf), ds_a, ve_a, b_a))" 
+                (evalF\<cdot>(Discr (?cnt, [], ve, nb b ?c)))| \<sqsubseteq>
+          \<aF>\<cdot>(Discr (PP (prim.If ct cf), ds_a, ve_a, b_a))"
     using ds_a by (subst HOLCFAbsCF.evalF.simps)(auto simp del:HOLCFAbsCF.evalF.simps)
   next
   fix ct cf cntt cntf
@@ -473,43 +455,43 @@ case (Next evalF evalC) {
   have new_elem: "|{((?c, [?c \<mapsto> b]), ?cnt)}| \<sqsubseteq> {((?c, [?c \<mapsto> b_a]), cont) |cont. cont \<in> ?cnt_a}"
     using abs_cntt and abs_cntf and abs_b by (auto simp add:sqsubset_is_subset)
 
-  have prem: "|(?cnt, [], ve, HOLCFExCF.nb b ?c)| \<sqsubseteq>
-              (contents |?cnt|, [], ve_a, contour_class.nb b_a ?c)"
+  have prem: "|(?cnt, [], ve, nb b ?c)| \<sqsubseteq>
+              (contents |?cnt|, [], ve_a, \<anb> b_a ?c)"
     using abs_ve and abs_cnt_nb[OF abs_b]
     by (simp)
-  have "|evalF\<cdot>(Discr (?cnt, [], ve, HOLCFExCF.nb b ?c))|
-       \<sqsubseteq> HOLCFAbsCF.evalF\<cdot>(Discr (contents |?cnt|, [], ve_a, contour_class.nb b_a ?c))"
+  have "|evalF\<cdot>(Discr (?cnt, [], ve, nb b ?c))|
+       \<sqsubseteq> \<aF>\<cdot>(Discr (contents |?cnt|, [], ve_a, \<anb> b_a ?c))"
     by (rule Next.hyps(1)[OF prem])
-  also have "\<dots> \<sqsubseteq> (\<Union>cnt\<in>?cnt_a. HOLCFAbsCF.evalF\<cdot>(Discr (cnt, [], ve_a, contour_class.nb b_a ?c)))"
+  also have "\<dots> \<sqsubseteq> (\<Union>cnt\<in>?cnt_a. \<aF>\<cdot>(Discr (cnt, [], ve_a, \<anb> b_a ?c)))"
     using abs_cntt and abs_cntf
     by (auto intro: contents_is_Proc[OF `isProc ?cnt`] simp del: evalF.simps simp add:sqsubset_is_subset)
 
   finally
-  have old_elems: "|evalF\<cdot>(Discr (?cnt, [], ve, HOLCFExCF.nb b ?c))|
-       \<sqsubseteq> (\<Union>cnt\<in>?cnt_a. HOLCFAbsCF.evalF\<cdot>(Discr (cnt, [], ve_a, contour_class.nb b_a ?c)))".
+  have old_elems: "|evalF\<cdot>(Discr (?cnt, [], ve, nb b ?c))|
+       \<sqsubseteq> (\<Union>cnt\<in>?cnt_a. \<aF>\<cdot>(Discr (cnt, [], ve_a, \<anb> b_a ?c)))".
 
-  have "|evalF\<cdot>(Discr (?cnt, [], ve, HOLCFExCF.nb b ?c))
+  have "|evalF\<cdot>(Discr (?cnt, [], ve, nb b ?c))
           \<union> {((?c, [?c \<mapsto> b]), ?cnt)}|
-        \<sqsubseteq> |evalF\<cdot>(Discr (?cnt, [], ve, HOLCFExCF.nb b ?c))|
+        \<sqsubseteq> |evalF\<cdot>(Discr (?cnt, [], ve, nb b ?c))|
           \<union> |{((?c, [?c \<mapsto> b]), ?cnt)}|"
     by (rule abs_ccache_union)
   also
   have "\<dots> \<sqsubseteq>
-        (\<Union>cnt\<in>?cnt_a. HOLCFAbsCF.evalF\<cdot>(Discr (cnt, [], ve_a, contour_class.nb b_a ?c)))
+        (\<Union>cnt\<in>?cnt_a. \<aF>\<cdot>(Discr (cnt, [], ve_a, \<anb> b_a ?c)))
         \<union> {((?c, [?c \<mapsto> b_a]), cont) |cont. cont \<in> ?cnt_a}"
     by (rule Un_mono_sq[OF old_elems new_elem])
   also
   have "\<dots> \<sqsubseteq> 
-        ((\<Union>cnt\<in>cntt_a. HOLCFAbsCF.evalF\<cdot>(Discr (cnt, [], ve_a, contour_class.nb b_a ct)))
+        ((\<Union>cnt\<in>cntt_a. \<aF>\<cdot>(Discr (cnt, [], ve_a, \<anb> b_a ct)))
           \<union> {((ct, [ct \<mapsto> b_a]), cont) |cont. cont \<in> cntt_a})
-      \<union> ((\<Union>cnt\<in>cntf_a. HOLCFAbsCF.evalF\<cdot>(Discr (cnt, [], ve_a, contour_class.nb b_a cf)))
+      \<union> ((\<Union>cnt\<in>cntf_a. \<aF>\<cdot>(Discr (cnt, [], ve_a, \<anb> b_a cf)))
           \<union> {((cf, [cf \<mapsto> b_a]), cont) |cont. cont \<in> cntf_a})"
     by (rule subst[OF sqsubset_is_subset[THEN sym],of "\<lambda>x. x",OF Un_upper1]
        |rule subst[OF sqsubset_is_subset[THEN sym],of "\<lambda>x. x",OF Un_upper2])
   finally
   show "|insert ((?c, [?c \<mapsto> b]), ?cnt)
-                (evalF\<cdot>(Discr (?cnt, [], ve, HOLCFExCF.nb b ?c)))| \<sqsubseteq>
-          HOLCFAbsCF.evalF\<cdot>(Discr (PP (prim.If ct cf), ds_a, ve_a, b_a))" 
+                (evalF\<cdot>(Discr (?cnt, [], ve, nb b ?c)))| \<sqsubseteq>
+          \<aF>\<cdot>(Discr (PP (prim.If ct cf), ds_a, ve_a, b_a))"
     using ds_a by (subst HOLCFAbsCF.evalF.simps)(auto simp del:HOLCFAbsCF.evalF.simps)
  qed
 next
@@ -528,116 +510,113 @@ case 2
 
   from cstate cstate_a abs_c abs_\<beta> abs_b
   show ?case
-  proof(cases c, auto simp add:HOL.Let_def simp del:evalF.simps evalC.simps set_map HOLCFExCF.evalV.simps)
+  proof(cases c, auto simp add:HOL.Let_def simp del:evalF.simps evalC.simps set_map evalV.simps)
 
   fix lab f vs
-  let ?d = "HOLCFExCF.evalV f \<beta> ve"
+  let ?d = "\<A> f \<beta> ve"
   assume "isProc ?d"
 
-  have "map (abs_d \<circ> (\<lambda>v. HOLCFExCF.evalV v \<beta> ve)) vs \<sqsubseteq> map (\<lambda>v. HOLCFAbsCF.evalV v \<beta>_a ve_a) vs"
+  have "map (abs_d \<circ> (\<lambda>v. \<A> v \<beta> ve)) vs \<sqsubseteq> map (\<lambda>v. \<aA> v \<beta>_a ve_a) vs"
     using abs_\<beta> and abs_d_evalV[OF abs_ve, of _ \<beta>]
     unfolding below_list_def
     by (auto intro!: list_all2I simp add:set_zip sqsubset_is_subset[THEN sym])
 
-  hence "|evalF\<cdot>(Discr (?d, map (\<lambda>v. HOLCFExCF.evalV v \<beta> ve) vs, ve, HOLCFExCF.nb b lab))|
-     \<sqsubseteq>  HOLCFAbsCF.evalF\<cdot>(Discr(contents |?d|, map (\<lambda>v. HOLCFAbsCF.evalV v \<beta>_a ve_a) vs, ve_a, contour_class.nb |b| lab))"
+  hence "|evalF\<cdot>(Discr (?d, map (\<lambda>v. \<A> v \<beta> ve) vs, ve, nb b lab))|
+     \<sqsubseteq>  \<aF>\<cdot>(Discr(contents |?d|, map (\<lambda>v. \<aA> v \<beta>_a ve_a) vs, ve_a, \<anb> |b| lab))"
     using abs_ve and abs_cnt_nb and abs_b
     by -(rule Next.hyps(1), auto)
-  also have "\<dots> \<sqsubseteq> (\<Union>f'\<in>HOLCFAbsCF.evalV f \<beta>_a ve_a.
-              HOLCFAbsCF.evalF\<cdot>(Discr(f', map (\<lambda>v. HOLCFAbsCF.evalV v \<beta>_a ve_a) vs, ve_a, contour_class.nb |b| lab)))"
+  also have "\<dots> \<sqsubseteq> (\<Union>f'\<in>\<aA> f \<beta>_a ve_a.
+              \<aF>\<cdot>(Discr(f', map (\<lambda>v. \<aA> v \<beta>_a ve_a) vs, ve_a, \<anb> |b| lab)))"
     using subsetD[OF abs_d_evalV[OF abs_ve] contents_is_Proc[OF `isProc ?d`]] and abs_\<beta>
     by (auto simp del: evalF.simps simp add:sqsubset_is_subset)
   finally
   have old_elems: "
-     |evalF\<cdot>(Discr (HOLCFExCF.evalV f \<beta> ve, map (\<lambda>v. HOLCFExCF.evalV v \<beta> ve) vs, ve, HOLCFExCF.nb b lab))|
-     \<sqsubseteq> (\<Union>f'\<in>HOLCFAbsCF.evalV f \<beta>_a ve_a.
-              HOLCFAbsCF.evalF\<cdot>(Discr(f', map (\<lambda>v. HOLCFAbsCF.evalV v \<beta>_a ve_a) vs, ve_a, contour_class.nb |b| lab)))"
+     |evalF\<cdot>(Discr (\<A> f \<beta> ve, map (\<lambda>v. \<A> v \<beta> ve) vs, ve, nb b lab))|
+     \<sqsubseteq> (\<Union>f'\<in> \<aA> f \<beta>_a ve_a.
+              \<aF>\<cdot>(Discr(f', map (\<lambda>v. \<aA> v \<beta>_a ve_a) vs, ve_a, \<anb> |b| lab)))"
     by auto
 
-  have new_elem: "|{((lab, \<beta>), HOLCFExCF.evalV f \<beta> ve)}|
-                  \<sqsubseteq> {((lab, \<beta>_a), f') |f'. f' \<in> HOLCFAbsCF.evalV f \<beta>_a ve_a}"
+  have new_elem: "|{((lab, \<beta>), \<A> f \<beta> ve)}|
+                  \<sqsubseteq> {((lab, \<beta>_a), f') |f'. f' \<in> \<aA> f \<beta>_a ve_a}"
     using abs_\<beta> and abs_d_evalV[OF abs_ve]
     by (auto simp add:sqsubset_is_subset)
     
-  have "|evalF\<cdot>(Discr (HOLCFExCF.evalV f \<beta> ve, map (\<lambda>v. HOLCFExCF.evalV v \<beta> ve) vs, ve, HOLCFExCF.nb b lab))
-        \<union> {((lab, \<beta>), HOLCFExCF.evalV f \<beta> ve)}|
-        \<sqsubseteq> |evalF\<cdot>(Discr (HOLCFExCF.evalV f \<beta> ve, map (\<lambda>v. HOLCFExCF.evalV v \<beta> ve) vs, ve, HOLCFExCF.nb b lab))|
-        \<union> |{((lab, \<beta>), HOLCFExCF.evalV f \<beta> ve)}|"
+  have "|evalF\<cdot>(Discr (\<A> f \<beta> ve, map (\<lambda>v. \<A> v \<beta> ve) vs, ve, nb b lab))
+        \<union> {((lab, \<beta>), \<A> f \<beta> ve)}|
+        \<sqsubseteq> |evalF\<cdot>(Discr (\<A> f \<beta> ve, map (\<lambda>v. \<A> v \<beta> ve) vs, ve, nb b lab))|
+        \<union> |{((lab, \<beta>), \<A> f \<beta> ve)}|"
     by (rule abs_ccache_union)
   also have "\<dots>
-        \<sqsubseteq> (\<Union>f'\<in>HOLCFAbsCF.evalV f \<beta>_a ve_a.
-              HOLCFAbsCF.evalF\<cdot>(Discr(f', map (\<lambda>v. HOLCFAbsCF.evalV v \<beta>_a ve_a) vs, ve_a, contour_class.nb |b| lab)))
-        \<union> {((lab, \<beta>_a), f') |f'. f' \<in> HOLCFAbsCF.evalV f \<beta>_a ve_a}"
+        \<sqsubseteq> (\<Union>f'\<in>\<aA> f \<beta>_a ve_a.
+              \<aF>\<cdot>(Discr(f', map (\<lambda>v. \<aA> v \<beta>_a ve_a) vs, ve_a, \<anb> |b| lab)))
+        \<union> {((lab, \<beta>_a), f') |f'. f' \<in> \<aA> f \<beta>_a ve_a}"
     by (rule Un_mono_sq[OF old_elems new_elem])
   finally
-  show "|insert ((lab, \<beta>), HOLCFExCF.evalV f \<beta> ve)
-                (evalF\<cdot>(Discr (HOLCFExCF.evalV f \<beta> ve, map (\<lambda>v. HOLCFExCF.evalV v \<beta> ve) vs, ve, HOLCFExCF.nb b lab)))|
-        \<sqsubseteq> HOLCFAbsCF.evalC\<cdot>(Discr (App lab f vs, |\<beta>|, ve_a, |b| ))"
+  show "|insert ((lab, \<beta>), \<A> f \<beta> ve)
+                (evalF\<cdot>(Discr (\<A> f \<beta> ve, map (\<lambda>v. \<A> v \<beta> ve) vs, ve, nb b lab)))|
+        \<sqsubseteq> \<aC>\<cdot>(Discr (App lab f vs, |\<beta>|, ve_a, |b| ))"
     using abs_\<beta>
     by (subst HOLCFAbsCF.evalC.simps)(auto simp add: HOL.Let_def simp del:HOLCFAbsCF.evalF.simps)
   next
   fix lab binds c'
 
-  have "|\<beta>(lab \<mapsto> HOLCFExCF.nb b lab)| =
-        \<beta>_a(lab \<mapsto> contour_class.nb |b| lab)"
+  have "|\<beta>(lab \<mapsto> nb b lab)| =
+        \<beta>_a(lab \<mapsto> \<anb> |b| lab)"
     using abs_\<beta> and abs_cnt_nb[OF abs_b] and abs_b
     by simp
   moreover
-  have "|map_of (map (\<lambda>(v, l). ((v, HOLCFExCF.nb b lab),
-                                 DC (l, \<beta>(lab \<mapsto> HOLCFExCF.nb b lab))))
+  have "|map_of (map (\<lambda>(v, l). ((v, nb b lab),
+                                 DC (l, \<beta>(lab \<mapsto> nb b lab))))
                      binds)|
-    \<sqsubseteq> smap_Union (map (\<lambda>(v, l).
-              smap_singleton (v, contour_class.nb |b| lab)
-               {PC (l, \<beta>_a(lab \<mapsto> contour_class.nb |b| lab))})
+    \<sqsubseteq> \<Union>. (map (\<lambda>(v, l).
+              {(v, \<anb> |b| lab) :=  {PC (l, \<beta>_a(lab \<mapsto> \<anb> |b| lab))}}.)
               binds)"
     using abs_cnt_nb[OF abs_b] and abs_b and abs_\<beta>
-    by  (auto intro:below_trans[OF abs_venv_map_of] smap_Union_mono list_all2I
+    by  (auto intro:below_trans[OF abs_venv_map_of] smap_union_mono list_all2I
               simp add:o_def set_zip abs_venv_singleton split_def)
   hence "|ve ++ map_of
             (map (\<lambda>(v, l).
-                   ((v, HOLCFExCF.nb b lab),
-                    DC (l, \<beta>(lab \<mapsto> HOLCFExCF.nb b lab))))
+                   ((v, nb b lab),
+                    DC (l, \<beta>(lab \<mapsto> nb b lab))))
                   binds)| \<sqsubseteq>
-       smap_union ve_a
-        (smap_Union
+        ve_a \<union>.
+        (\<Union>.
           (map (\<lambda>(v, l).
-                   smap_singleton (v, contour_class.nb |b| lab)
-                    {PC (l, \<beta>_a(lab \<mapsto> contour_class.nb |b| lab))})
+            {(v, \<anb> |b| lab) :=  {PC (l, \<beta>_a(lab \<mapsto> \<anb> |b| lab))}}.)
             binds))"
     by (rule below_trans[OF abs_venv_union, OF smap_union_mono[OF abs_ve]])
   ultimately
-  have "|evalC\<cdot>(Discr(c', \<beta>(lab \<mapsto> HOLCFExCF.nb b lab),
+  have "|evalC\<cdot>(Discr(c', \<beta>(lab \<mapsto> nb b lab),
             ve ++ map_of
-                  (map (\<lambda>(v, l). ((v, HOLCFExCF.nb b lab), DC (l, \<beta>(lab \<mapsto> HOLCFExCF.nb b lab)))) binds),
-            HOLCFExCF.nb b lab))|
-    \<sqsubseteq> HOLCFAbsCF.evalC\<cdot>(Discr (c', \<beta>_a(lab \<mapsto> contour_class.nb |b| lab),
-            smap_union ve_a
-             (smap_Union (map (\<lambda>(v, l).
-                   smap_singleton (v, contour_class.nb |b| lab)
-                    {PC (l, \<beta>_a(lab \<mapsto> contour_class.nb |b| lab))})
-                            binds)),
-         contour_class.nb |b| lab))"
+                  (map (\<lambda>(v, l). ((v, nb b lab), DC (l, \<beta>(lab \<mapsto> nb b lab)))) binds),
+            nb b lab))|
+    \<sqsubseteq> \<aC>\<cdot>(Discr (c', \<beta>_a(lab \<mapsto> \<anb> |b| lab),
+            ve_a \<union>.
+             (\<Union>. (map (\<lambda>(v, l).
+                   {(v, \<anb> |b| lab) :=  {PC (l, \<beta>_a(lab \<mapsto> \<anb> |b| lab))}}.)
+                   binds)),
+         \<anb> |b| lab))"
     using abs_cnt_nb and abs_b
     by -(rule Next.hyps(2),auto intro:abs_cnt_nb[OF abs_b])
 
-  thus "|evalC\<cdot>(Discr (c', \<beta>(lab \<mapsto> HOLCFExCF.nb b lab),
-                      ve ++ map_of (map (\<lambda>(v, l).((v, HOLCFExCF.nb b lab),HOLCFExCF.evalV (L l) (\<beta>(lab \<mapsto> HOLCFExCF.nb b lab)) ve)) binds),
-                      HOLCFExCF.nb b lab))| \<sqsubseteq>
-          HOLCFAbsCF.evalC\<cdot>(Discr (call.Let lab binds c', |\<beta>|, ve_a, |b| ))"
+  thus "|evalC\<cdot>(Discr (c', \<beta>(lab \<mapsto> nb b lab),
+                      ve ++ map_of (map (\<lambda>(v, l).((v, nb b lab),\<A> (L l) (\<beta>(lab \<mapsto> nb b lab)) ve)) binds),
+                      nb b lab))| \<sqsubseteq>
+          \<aC>\<cdot>(Discr (call.Let lab binds c', |\<beta>|, ve_a, |b| ))"
     using abs_\<beta>
     by (subst HOLCFAbsCF.evalC.simps)(auto simp add: HOL.Let_def simp del:HOLCFAbsCF.evalC.simps)
   qed
 }
 qed
 
-definition evalCPS :: "prog \<Rightarrow> ('c::contour) ans"
-  where "evalCPS l = (let ve = smap_empty;
+definition evalCPS_a :: "prog \<Rightarrow> ('c::contour) ans" ("\<aPR>")
+  where "\<aPR> l = (let ve = {}.;
                           \<beta> = empty;
-                          f = evalV (L l) \<beta> ve
-                      in  evalF\<cdot>(Discr (contents f,[{Stop}],ve,initial_contour)))"
+                          f = \<aA> (L l) \<beta> ve
+                      in  \<aF>\<cdot>(Discr (contents f,[{Stop}],ve,\<abinit>)))"
 
-lemma lemma6: "|HOLCFExCF.evalCPS l| \<sqsubseteq> evalCPS l"
-  unfolding HOLCFExCF.evalCPS_def evalCPS_def
+lemma lemma6: "|\<PR> l| \<sqsubseteq> \<aPR> l"
+  unfolding evalCPS_def evalCPS_a_def
   by (auto intro:lemma89 simp del:evalF.simps HOLCFExCF.evalF.simps)
   
 end
